pre-reu

theories/STLC/Layered.v
@@ -23,52 +23,122 @@ Variant kont : Type :=
 | KVar : neg_ty -> kont
 .
 
+Definition k_ctx : Type := Ctx.ctx kont.
+Bind Scope ctx_scope with k_ctx.
+
 Equations k_move : kont -> Type :=
   k_move (KCtx x) := a_val x ;
   k_move (KVar x) := t_obs x .
 
-Equations k_next (k : kont) : k_move k -> list kont :=
-  k_next (KCtx x) a := map KVar (a_cext a) ;
-  k_next (KVar x) o := cons (KCtx (t_obs_goal o)) (map KVar (t_obs_args o)) .
+Definition lassen_c_ix : Type := frame .
+Definition lassen_s_ix : Type := (frame + neg_ctx) * frame .
+
+Equations lassen_c_move : lassen_c_ix -> Type :=
+  lassen_c_move c_i := any t_obs (fst c_i) + a_val (snd c_i) .
+
+Equations lassen_c_next c_i : lassen_c_move c_i -> lassen_s_ix :=
+  lassen_c_next c_i (inl a) := (inl (any_elim (@t_obs_nxt) _ a) , c_i) ;
+  lassen_c_next c_i (inr a) := (inr (a_cext a) , c_i) .
+
+Equations lassen_s_move : lassen_s_ix -> Type :=
+  lassen_s_move (inl s_i , _) := any t_obs (fst s_i) + a_val (snd s_i) ;
+  lassen_s_move (inr s_i , _) := any t_obs s_i .
+
+Equations lassen_s_next s_i : lassen_s_move s_i -> lassen_c_ix :=
+  lassen_s_next (inl s_i , c_i) (inl a) :=
+    ((fst c_i +▶ any_elim (@t_obs_args) _ a)%ctx ,
+     any_elim (@t_obs_goal) _ a) ;
+  lassen_s_next (inl s_i , c_i) (inr a) := ((fst c_i +▶ a_cext a)%ctx , snd c_i) ;
+  lassen_s_next (inr s_i , c_i) a :=
+    ((fst c_i +▶ any_elim (@t_obs_args) _ a)%ctx ,
+     any_elim (@t_obs_goal) _ a) .
+
+Definition g_lassen : game' lassen_c_ix lassen_s_ix :=
+  {| client := {| move := lassen_c_move ;
+                  next := lassen_c_next |} ;
+     server := {| move := lassen_s_move ;
+                  next := lassen_s_next |} |} .
 
 (*
-Definition base : half_game (list kont) (list kont) :=
-  {| move := any k_move ;
-     next := any_elim k_next |} .
+Definition kctx_of_nctx (Γ : neg_ctx) : k_ctx := map KVar Γ .
+Definition kctx_of_frame (s : frame) : k_ctx := kctx_of_nctx (fst s) ▶ KCtx (snd s).
 
-Definition g_lassen : game' (list kont) (list kont * list kont) :=
-  {| client := {| move := fun xs => any k_move xs ;
-                  next := fun xs m => (any_elim k_next xs m , xs) |} ;
-     server := {| move := fun ys => any k_move (fst ys) ;
-                  next := fun ys m => app (any_elim k_next (fst ys) m) (snd ys) |} |} .
+Variant k_ext : Type :=
+| KPush : frame -> k_ext
+| KPop : neg_ctx -> k_ext
+.
+
+Equations kctx_of_kext : k_ext -> k_ctx :=
+  kctx_of_kext (KPush s) := kctx_of_frame s ;
+  kctx_of_kext (KPop Δ)  := kctx_of_nctx Δ .
+
+Definition ext_kctx (ks : k_ctx) (e : k_ext) : k_ctx
+  := ks +▶ kctx_of_kext e.
+
+Equations ext_frame : frame -> k_ext -> frame :=
+  ext_frame u (KPush v) := ((fst u +▶ fst v)%ctx , snd v) ;
+  ext_frame u (KPop Γ)  := ((fst u +▶ Γ)%ctx , snd u) .
+
+Equations k_next (k : kont) : k_move k -> k_ext :=
+  k_next (KCtx x) a := KPop (a_cext a) ;
+  k_next (KVar x) o := KPush (t_obs_nxt o) .
+
+Definition g_lassen : game' frame (k_ctx * frame) :=
+  {| client := {| move := fun i => any k_move (kctx_of_frame i) ;
+                  next := fun i m => (kctx_of_kext (any_elim k_next _ m) , i) |} ;
+     server := {| move := fun i => any k_move (fst i) ;
+                  next := fun i m => ext_frame (snd i) (any_elim k_next _ m) |} |} .
+
+Equations inj_ogs_enf {s} : e_nf' s -> itree g_lassen (eval_arg' +ᵢ ∅ᵢ) s :=
+  inj_ogs_enf (NVal v) := Vis (Any _ _ top (a_of_val v) : qry g_lassen _) _ ;
+  inj_ogs_enf (NRed E i v) := _ .
+
+  destruct s as [Γ x]; intros [ v | ? ? E i e ]; cbn in *.
+  + unshelve refine (Vis (Any _ _ top _ : qry g_lassen _) _).
+    refine (a_of_val v).
+    intros [k i m]; cbn in i |- *.
+    revert m.
+    rewrite <- (has_map2 _ _ i).
+    intros m. cbn in m. cbn.
+    refine (Ret (inl _)).
+    refine (earg_start (t_obs_apply m (cext_get _ v (has_map1 _ _ i)))).
+  + unshelve refine (Vis _ _).
+    destruct (neg_var i).
+    refine (Any _ _ (pop _) _). refine (map_has KVar _ (has_map1 _ _ i)).
+    cbn. Check (has_map2 of_n_ty Γ i).
+    cbn.
+    cbn. Check (t)
+    cbn. Check (cext_get).
+    destruct r.
+    dependent elimination x0.
+    - shelve.
+
 *)
 
-Definition half_ogs : half_game (list kont * list kont) (list kont * list kont) :=
-  {| move := fun xs => any k_move (fst xs) ;
-     next := fun xs m => (app (any_elim k_next _ m) (snd xs) , fst xs) |} .
+Definition half_ogs : half_game (k_ctx * k_ctx) (k_ctx * k_ctx) :=
+  {| move := fun i => any k_move (fst i) ;
+     next := fun i m => (ext_kctx (snd i) (any_elim k_next _ m) , fst i) |} .
 
-Definition g_ogs : game' (list kont * list kont) (list kont * list kont) :=
+Definition g_ogs : game' (k_ctx * k_ctx) (k_ctx * k_ctx) :=
   {| client := half_ogs ; server := half_ogs |}.
 
 Definition ogs := itree g_ogs ∅ᵢ.
 
 Section composition.
-  
-Variant _compo_arg (showₚ showₒ hideₚ hideₒ fullₚ fullₒ : list kont) : Type :=
-| _c_ap  : ogs (fullₚ , fullₒ)
-         -> iforest g_ogs ∅ᵢ (hideₚ , hideₒ)
-         -> _compo_arg showₚ showₒ hideₚ hideₒ fullₚ fullₒ
-| _c_pa : iforest g_ogs ∅ᵢ (fullₒ , fullₚ)
-        -> ogs (hideₒ , hideₚ)
-        -> _compo_arg showₚ showₒ hideₚ hideₒ fullₚ fullₒ
+
+Variant _compo_arg (hideₚ hideₒ fullₚ fullₒ : k_ctx) : Type :=
+| _c_ap  : ogs (fullₚ , fullₒ) -> iforest g_ogs ∅ᵢ (hideₚ , hideₒ)
+         -> _compo_arg hideₚ hideₒ fullₚ fullₒ
+| _c_pa : iforest g_ogs ∅ᵢ (fullₒ , fullₚ) -> ogs (hideₒ , hideₚ)
+        -> _compo_arg hideₚ hideₒ fullₚ fullₒ
   .
-Arguments _c_pa {showₚ showₒ hideₚ hideₒ fullₚ fullₒ} a b.
-Arguments _c_ap {showₚ showₒ hideₚ hideₒ fullₚ fullₒ} a b.
+Arguments _c_pa {hideₚ hideₒ fullₚ fullₒ} a b.
+Arguments _c_ap {hideₚ hideₒ fullₚ fullₒ} a b.
 
 Definition _compo : forall showₚ showₒ hideₚ hideₒ fullₚ fullₒ
                     , showₚ ⊎ hideₚ ≡ fullₚ
                     -> showₒ ⊎ hideₒ ≡ fullₒ
-                    -> _compo_arg showₚ showₒ hideₚ hideₒ fullₚ fullₒ
+                    -> _compo_arg hideₚ hideₒ fullₚ fullₒ
                     -> ogs (showₚ , showₒ).
   cofix CIH.
   intros ? ? ? ? ? ? cₚ cₒ [a b|a b].
@@ -92,46 +162,41 @@ Definition _compo : forall showₚ showₒ hideₚ hideₒ fullₚ fullₒ
 Defined.
 Arguments _compo {_ _ _ _ _ _}.
 
-Definition compo_ap {showₚ showₒ hideₚ hideₒ fullₚ fullₒ}
-      (cₚ : showₚ ⊎ hideₚ ≡ fullₚ) (cₒ : showₒ ⊎ hideₒ ≡ fullₒ)
-      (a : ogs (fullₚ , fullₒ)) (b : iforest g_ogs ∅ᵢ (hideₚ , hideₒ))
-      : ogs (showₚ , showₒ)
-  := _compo cₚ cₒ (_c_ap a b).
+Definition compo_ap {sₚ sₒ hₚ hₒ fₚ fₒ} (cₚ : sₚ ⊎ hₚ ≡ fₚ) (cₒ : sₒ ⊎ hₒ ≡ fₒ)
+      := fun a b => _compo cₚ cₒ (_c_ap a b).
 
-Definition compo_pa {showₚ showₒ hideₚ hideₒ fullₚ fullₒ}
-      (cₚ : showₚ ⊎ hideₚ ≡ fullₚ) (cₒ : showₒ ⊎ hideₒ ≡ fullₒ)
-      (a : iforest g_ogs ∅ᵢ (fullₒ , fullₚ)) (b : ogs (hideₒ , hideₚ))
-      : ogs (showₚ , showₒ)
-  := _compo cₚ cₒ (_c_pa a b).
+Definition compo_pa {sₚ sₒ hₚ hₒ fₚ fₒ} (cₚ : sₚ ⊎ hₚ ≡ fₚ) (cₒ : sₒ ⊎ hₒ ≡ fₒ)
+      := fun a b => _compo cₚ cₒ (_c_pa a b).
+Check compo_ap.
 
 (**********)
 (* PROOFS *)
 (**********)
 
 
-Variant _compo_arg_eq (showₚ showₒ hideₚ hideₒ fullₚ fullₒ : list kont) : Type :=
+Variant _compo_arg_eq (hideₚ hideₒ fullₚ fullₒ : list kont) : Type :=
 | _c_pa2 (a0 a1 : iforest g_ogs ∅ᵢ (fullₒ , fullₚ)) (b0 b1 : ogs (hideₒ , hideₚ))
-  : (forall r, a0 r ≈ a1 r) -> b0 ≈ b1 -> _compo_arg_eq showₚ showₒ hideₚ hideₒ fullₚ fullₒ 
+  : (forall r, a0 r ≈ a1 r) -> b0 ≈ b1 -> _compo_arg_eq hideₚ hideₒ fullₚ fullₒ 
 | _c_ap2 (a0 a1 : ogs (fullₚ , fullₒ)) (b0 b1 : iforest g_ogs ∅ᵢ (hideₚ , hideₒ))
-  : a0 ≈ a1 -> (forall r, b0 r ≈ b1 r) -> _compo_arg_eq showₚ showₒ hideₚ hideₒ fullₚ fullₒ 
+  : a0 ≈ a1 -> (forall r, b0 r ≈ b1 r) -> _compo_arg_eq hideₚ hideₒ fullₚ fullₒ 
   .
-Arguments _c_pa2 {showₚ showₒ hideₚ hideₒ fullₚ fullₒ} a0 a1 b0 b1 ea eb.
-Arguments _c_ap2 {showₚ showₒ hideₚ hideₒ fullₚ fullₒ} a0 a1 b0 b1 ea eb.
+Arguments _c_pa2 {hideₚ hideₒ fullₚ fullₒ} a0 a1 b0 b1 ea eb.
+Arguments _c_ap2 {hideₚ hideₒ fullₚ fullₒ} a0 a1 b0 b1 ea eb.
 
-Equations _c_arg_eq_l {sₚ sₒ hₚ hₒ fₚ fₒ}
-  : _compo_arg_eq sₚ sₒ hₚ hₒ fₚ fₒ -> _compo_arg sₚ sₒ hₚ hₒ fₚ fₒ :=
+Equations _c_arg_eq_l {hₚ hₒ fₚ fₒ} : _compo_arg_eq hₚ hₒ fₚ fₒ
+                                    -> _compo_arg hₚ hₒ fₚ fₒ :=
   _c_arg_eq_l (_c_pa2 a0 a1 b0 b1 ea eb) := _c_pa a0 b0 ;
   _c_arg_eq_l (_c_ap2 a0 a1 b0 b1 ea eb) := _c_ap a0 b0 .
     
-Equations _c_arg_eq_r {sₚ sₒ hₚ hₒ fₚ fₒ}
-  : _compo_arg_eq sₚ sₒ hₚ hₒ fₚ fₒ -> _compo_arg sₚ sₒ hₚ hₒ fₚ fₒ :=
+Equations _c_arg_eq_r {hₚ hₒ fₚ fₒ} : _compo_arg_eq hₚ hₒ fₚ fₒ
+                                    -> _compo_arg hₚ hₒ fₚ fₒ :=
   _c_arg_eq_r (_c_pa2 a0 a1 b0 b1 ea eb) := _c_pa a1 b1 ;
   _c_arg_eq_r (_c_ap2 a0 a1 b0 b1 ea eb) := _c_ap a1 b1 .
     
 
 (* bisimilarity of composition of pairwise bisimilar arguments *)
 Lemma _compo_cong {sₚ sₒ hₚ hₒ fₚ fₒ} (cₚ : sₚ ⊎ hₚ ≡ fₚ) (cₒ : sₒ ⊎ hₒ ≡ fₒ)
-      (a : _compo_arg_eq sₚ sₒ hₚ hₒ fₚ fₒ)
+      (a : _compo_arg_eq hₚ hₒ fₚ fₒ)
       : _compo cₚ cₒ (_c_arg_eq_l a) ≈ _compo cₚ cₒ (_c_arg_eq_r a).
   revert sₚ sₒ hₚ hₒ fₚ fₒ cₚ cₒ a.
   pcofix CIH; pstep.
@@ -179,7 +244,6 @@ Check _compo_cong.
 
 (***
 lem1 : norm a ≈ norm b -> inj_ogs a ≈ inj_ogs b
-lem2 : inj_ogs a ≈ inj_ogs b -> norm a ≈ norm b
 
 a ≈obs b := forall E, norm (E[a]) ≈ norm (E[b]) 
 
